src/Init/Data/Iterators/Consumers/Monadic/Collect.lean
@@ -9,7 +9,7 @@ prelude
 public import Init.Data.Iterators.Consumers.Monadic.Partial
 public import Init.Data.Iterators.Consumers.Monadic.Total
 public import Init.Data.Iterators.Internal.LawfulMonadLiftFunction
-public import Init.Internal.ExtrinsicTermination
+public import Init.WFExtrinsicFix
 
 @[expose] public section
 
@@ -82,43 +82,13 @@ where
   @[always_inline]
   go it (acc : Array γ) : n (Array γ) :=
     letI : MonadLift m n := ⟨lift (α := _)⟩
-    extrinsicFix₂ (C₂ := fun _ _ => n (Array γ)) (InvImage TerminationMeasures.Finite.Rel (·.1.finitelyManySteps!))
+    WellFounded.extrinsicFix₂ (C₂ := fun _ _ => n (Array γ)) (InvImage TerminationMeasures.Finite.Rel (·.1.finitelyManySteps!))
     (fun (it : IterM (α := α) m β) acc recur => do
       match (← it.step).inflate with
       | .yield it' out h =>
         recur it' (acc.push (← f out)) (by exact TerminationMeasures.Finite.rel_of_yield ‹_›)
       | .skip it' h => recur it' acc (by exact TerminationMeasures.Finite.rel_of_skip ‹_›)
       | .done _ => return acc) it acc
-
--- @[always_inline, no_expose]
--- def IterM.DefaultConsumers.toArrayMapped {α β : Type w} {m : Type w → Type w'}
---     {n : Type w → Type w''} [Monad n] [MonadAttach n] [Iterator α m β]
---     (lift : ⦃α : Type w⦄ → m α → n α) {γ : Type w} (f : β → n γ)
---     (it : IterM (α := α) m β) : n (Array γ) :=
---   letI : MonadLift m n := ⟨lift (α := _)⟩
---   go it #[]
--- where
---   @[always_inline]
---   go it (acc : Array γ) : n (Array γ) :=
---     letI : MonadLift m n := ⟨lift (α := _)⟩
---     extrinsicFix₂ (C₂ := fun _ _ => n (Array γ))
---     (fun x' x => (∃ out, x.1.IsPlausibleStepE (.yield x'.1 out) ∧ ∃ fx, MonadAttach.CanReturn (f out) fx ∧ x'.2 = x.2.push fx) ∨ (∃ h, MonadAttach.CanReturn (m := n) x.1.step (.deflate <| .skip x'.1 h) ∧ x'.2 = x.2))
---     (fun (it : IterM (α := α) m β) acc recur => do
---       let ⟨step, hs⟩ ← MonadAttach.attach (m := n) it.step
---       match hs' : step.inflate with
---       | .yield it' out h =>
---         let fx ← MonadAttach.attach (f out)
---         recur it' (acc.push fx.val) (by
---           apply Or.inl
---           have : step = .deflate (.yield it' out h) := by simp [← hs']
---           rw [this] at hs
---           exact ⟨out, h, hs, fx.val, fx.property, rfl⟩)
---       | .skip it' h => recur it' acc (by
---           apply Or.inr
---           have : step = .deflate (.skip it' h) := by simp [← hs']
---           rw [this] at hs
---           exact ⟨h, hs, rfl⟩)
---       | .done h => return acc) it acc
 
 /--
 This is the default implementation of the `IteratorCollect` class.
@@ -208,7 +178,7 @@ def IterM.toListRev {α : Type w} {m : Type w → Type w'} [Monad m] {β : Type 
 where
   @[always_inline, inline]
   go (it : IterM m β) acc :=
-    extrinsicFix₂ (InvImage TerminationMeasures.Finite.Rel (·.1.finitelyManySteps!))
+    WellFounded.extrinsicFix₂ (InvImage TerminationMeasures.Finite.Rel (·.1.finitelyManySteps!))
       (fun it acc recur => do
         match (← it.step).inflate with
         | .yield it' out h => recur it' (out :: acc) (TerminationMeasures.Finite.rel_of_yield h)
